Make an example of echo output n times
After     | File Name              | Before    || Change
-----------------------------------------------------------
10m18.59s | Total                  | 10m15.06s || +0m03.52s
-----------------------------------------------------------
0m30.80s  | examples/specexamples  | 0m26.44s  || +0m04.35s
0m26.58s  | x86/instrrules/cmp     | 0m28.61s  || -0m02.03s
0m18.20s  | x86/instrrules/callrel | 0m19.83s  || -0m01.62s
0m41.31s  | x86/instrrules/addsub  | 0m41.33s  || -0m00.01s
0m31.96s  | x86/instrrules/core    | 0m31.29s  || +0m00.67s
0m30.76s  | examples/mulc          | 0m31.10s  || -0m00.33s
0m21.28s  | x86/instrrules/shift   | 0m21.33s  || -0m00.04s
0m20.78s  | x86/cfuncspec          | 0m20.71s  || +0m00.07s
0m20.71s  | x86/listproof          | 0m20.70s  || +0m00.01s
0m19.44s  | x86/instrrules/adc     | 0m18.87s  || +0m00.57s
0m18.92s  | x86/macros             | 0m18.76s  || +0m00.16s
0m18.54s  | x86/instrrules/and     | 0m18.48s  || +0m00.05s
0m17.28s  | x86/call               | 0m17.00s  || +0m00.28s
0m17.09s  | x86/instrrules/mov     | 0m16.89s  || +0m00.19s
0m15.96s  | x86/inlinealloc        | 0m16.08s  || -0m00.11s
0m15.68s  | x86/imp                | 0m15.50s  || +0m00.17s
0m15.21s  | x86/main               | 0m14.69s  || +0m00.52s
0m14.29s  | x86/wrapalloc          | 0m13.67s  || +0m00.61s
0m14.13s  | x86/lifeimp            | 0m14.95s  || -0m00.81s
0m13.47s  | x86/instrrules/jmprel  | 0m13.51s  || -0m00.03s
0m13.28s  | x86/instrrules/incdec  | 0m13.74s  || -0m00.46s
0m12.74s  | x86/screenproof        | 0m11.99s  || +0m00.75s
0m09.88s  | x86/instrrules/pop     | 0m09.90s  || -0m00.01s
0m09.81s  | x86/instrrules/push    | 0m10.09s  || -0m00.27s
0m09.24s  | x86/cstringimp         | 0m09.17s  || +0m00.07s
0m08.38s  | examples/xorswap       | 0m08.40s  || -0m00.01s
0m08.16s  | x86/instrrules/xor     | 0m08.07s  || +0m00.08s
0m07.36s  | x86/basicprog          | 0m07.61s  || -0m00.25s
0m07.07s  | x86/instrrules/not     | 0m07.00s  || +0m00.07s
0m06.83s  | x86/gcdex              | 0m06.40s  || +0m00.42s
0m06.75s  | x86/instrrules/or      | 0m06.58s  || +0m00.16s
0m06.21s  | x86/instrrules/neg     | 0m06.10s  || +0m00.11s
0m05.69s  | examples/fact          | 0m05.50s  || +0m00.19s
0m05.64s  | x86/testrun            | 0m05.23s  || +0m00.40s
0m05.62s  | x86/instrrules/jccrel  | 0m05.55s  || +0m00.07s
0m05.56s  | x86/screenspec         | 0m05.37s  || +0m00.18s
0m05.54s  | x86/screenimp          | 0m05.38s  || +0m00.16s
0m05.43s  | x86/instrrules/test    | 0m05.47s  || -0m00.04s
0m05.42s  | x86/listimp            | 0m05.36s  || +0m00.05s
0m05.42s  | x86/instrrules/ret     | 0m05.49s  || -0m00.07s
0m05.35s  | x86/listspec           | 0m05.41s  || -0m00.06s
0m05.35s  | x86/cfunc              | 0m05.12s  || +0m00.22s
0m05.24s  | x86/instrrules/lea     | 0m05.33s  || -0m00.08s
0m05.18s  | x86/instrrules/in      | 0m05.61s  || -0m00.43s
0m05.08s  | basicspectac           | 0m04.80s  || +0m00.28s
0m05.05s  | x86/examples           | 0m05.19s  || -0m00.14s
0m05.00s  | x86/instrrules         | 0m05.09s  || -0m00.08s
0m04.97s  | x86/instrrules/out     | 0m05.06s  || -0m00.08s
0m04.95s  | examples/entry         | 0m05.32s  || -0m00.37s

src/examples/specexamples.v
@@ -287,3 +287,78 @@ Proof.
   eapply safe_loop_forever_constant.
   do_basic'.
 Qed.
+
+Definition echo_once in_c out_c :=
+  (IN in_c, AL;;
+   OUT out_c, AL).
+
+Definition echo_once_clean (al in_c out_c : BYTE) :=
+  (echo_once in_c out_c;;
+   MOV AL, al).
+
+Definition echo_once_OP_helper (in_c out_c : BYTE) v := catOP (inOP (zeroExtend n8 in_c) v) (outOP (zeroExtend n8 out_c) v).
+
+Example safe_echo_once al in_c out_c
+: |-- Forall v, basic (BYTEregIs AL al)
+                      (echo_once in_c out_c)
+                      (echo_once_OP_helper in_c out_c v)
+                      (BYTEregIs AL v).
+Proof.
+  specintros => v. rewrite /echo_once/echo_once_OP_helper.
+  do_basic'; first by reflexivity.
+  do_basic'.
+Qed.
+
+Instance: forall in_c out_c, instrrule (echo_once in_c out_c) := fun in_c out_c al => @safe_echo_once al in_c out_c.
+
+Example safe_echo_once_clean (al in_c out_c : BYTE) v
+: |-- (basic (BYTEregIs AL al)
+             (echo_once_clean al in_c out_c)
+             (echo_once_OP_helper in_c out_c v)
+             (BYTEregIs AL al)).
+Proof.
+  rewrite /echo_once_clean/echo_once_OP_helper.
+  do_basic'.
+  do_basic'.
+  rewrite low_catB. by ssimpl.
+Qed.
+
+Instance: forall al in_c out_c, instrrule (echo_once_clean al in_c out_c) := @safe_echo_once_clean.
+
+Definition echo_n al in_c out_c n := output_n_prog (echo_once_clean al in_c out_c) n.
+
+Definition list_to_in_out (in_c out_c : BYTE) ls
+  := [seq catOP (inOP (zeroExtend n8 in_c) v) (outOP (zeroExtend n8 out_c) v) | v <- ls ].
+
+(** TODO: clean up this proof *)
+Example safe_echo_n in_c out_c n d
+        (small_enough : nat -> Prop)
+        (is_small : forall n, small_enough (n.+1) -> small_enough n)
+        (small_is_good : forall n, small_enough n -> (#(n.+1) == @fromNat n32 0) = false)
+        (Hn : small_enough n)
+: |-- Forall ls (pf : n.+1 < size ls),
+  (basic (ECX ~= #n ** BYTEregIs AL d)
+         (echo_n d in_c out_c n)
+         (rollOP n (fun k => nth empOP (list_to_in_out in_c out_c ls) (k.-1)))
+         (ECX ~= #0 ** BYTEregIs AL d)
+         @ OSZCP?).
+Proof.
+  specintros => ls pf.
+  rewrite /echo_n.
+  pose proof (@safe_loop_n (fun _ => empSP) (echo_once_clean d in_c out_c) (fun k => nth empOP (list_to_in_out in_c out_c ls) (k.-1)) n d (fun k => small_enough k /\ k < n.+1)) as H.
+  cbv beta in H.
+  rewrite -> !empSPR in H.
+  apply H; [ by intuition | by intuition | by intuition | ].
+  move => n' [ Hsmall Hle ].
+  clear H.
+  pre_basic_apply;
+    (let R := get_next_instrrule_for_basic in
+     try_basicapply R).
+  simpl.
+  rewrite /echo_once_OP_helper.
+  rewrite /list_to_in_out.
+  erewrite nth_map; first by reflexivity.
+  by erewrite ltn_trans; try eassumption.
+  Grab Existential Variables.
+  exact #0.
+Qed.
